Theorem8.v
@@ -16,8 +16,162 @@ Require Import contract_definition.
 Require Import contract_subs.
 Require Import contract_Eval.
 Require Import lemma5.
+Require Import Theorem7_Lemma.
 Require Import Theorem7.
+Require Import Omega.
 Import parameters.
 Import Operational_Semantics.
 
-Theorem Theorem8: forall (Ex Ex':Exec) (θ θ:Store), WF Ex -> CausCons θ Ex -> 
+
+Lemma Theorem8_dom_help : forall η θ r,  dom (F_Union θ r η) = Singleton ReplID r.
+Proof.
+intros.
+compute. admit.
+Qed.
+
+
+Lemma Theorem8_nat_help : forall i:SeqNo, (i<>0) -> (lt (i-1) i).
+Proof.
+  intros.
+  destruct i. 
+  -compute in H. assert (0=0). reflexivity. intuition.
+  - omega.
+Qed.
+  
+Lemma  Theorem8_beq_help:  forall η θ r,  F_Union θ r η r = Union Effect ( θ r) (Singleton Effect η).
+  Proof. admit. Qed.
+
+  
+Theorem Theorem8: forall Σ Ex Ex' θ θ' η τ Ing1 Ing2 ss ii σσ op, 
+                     (Ing1 = (mkSoup_Ing ss ii ((mkop_cls op τ)::σσ))) ->
+                     (Ing2 = (mkSoup_Ing ss (ii+1) σσ)) ->
+                     (WF_union Σ Ing1) -> (WF_union Σ Ing2) ->
+                     [[Ex,θ,(Σ||| Ing1) --τ,η-->  Ex' ,θ' , (Σ|||Ing2)]] ->
+
+                     WF Ex -> CausCons θ Ex -> CausCons θ' Ex'.
+Proof. intros  Σ Ex Ex' θ θ' η τ Ing1 Ing2 ss ii σσ op HIng1 HIng2. intros HWF_Union1 HWF_Union2.
+       intros HProg HWF HCausCons.
+       inversion HProg; subst.
+       -Case"EffVis". rename Ex' into Ex. clear H. 
+        unfold CausCons. intros; rename η0 into η'; rename r0 into r'.
+        rename H into HAa. rename H0 into H. rename H1 into H0. rename H2 into H1. rename H3 into H2.
+        rename H4 into H3. rename H5 into H4. rename H6 into H5. rename H7 into H6. 
+        inversion H; subst.
+        +destruct H7.  unfold CausCons in HCausCons. specialize (HCausCons r' a η').
+         apply HCausCons; auto. 
+         
+         
+
+
+
+         
+        +inversion H7. rewrite H7. rewrite<- H7 in H4. rewrite Theorem8_dom_help in H4. destruct H4.
+         (*nice so far*)
+         rewrite <- H8 in H5.
+         rewrite Theorem8_beq_help in H5.
+         inversion H5.
+         (*1- η' is in θr*)
+         subst.
+         rewrite Theorem8_beq_help. apply Union_introl. compute.
+         unfold CausCons in HCausCons. specialize (HCausCons r a η').
+         apply HCausCons;auto. 
+         (*2  η'=η*)
+         inversion H4; subst; rename η' into η.
+         destruct Ex as [A vis so sameobj]. 
+         apply Inversion_HBO_Help with (A:=A) (vis:=vis) (so:=so) (sameobj:=sameobj)in H6.
+         destruct H6 as [|Hsingle]. rename H6 into Hsteps.
+         (***2.1 multiple steps behind hbo*)
+         destruct Hsteps as [c]. destruct H6 as [HBOac Hsinglecη].
+         assert (θ r c). { 
+            apply H2. unfold In. simpl. destruct Hsinglecη.
+            apply Union_introl. unfold In. apply first. apply H6.
+            apply Union_intror. destruct H6. unfold In. apply first. apply H6. }
+         
+         rewrite Theorem8_beq_help. apply Union_introl.
+         unfold In. unfold CausCons in HCausCons.
+         specialize (HCausCons r a c). apply HCausCons; auto. 
+         (***2.2 ONE step behind hbo*)
+         (*2.2.1 from so*)
+         rewrite Theorem8_beq_help. apply Union_introl.
+         apply H2. unfold In.  simpl.
+         destruct Hsingle.  apply Union_intror.
+         unfold In. apply first. inversion H6. apply H8.
+         (*2.2.2 from vis*)
+         apply Union_introl. unfold In. apply first. apply H6.
+         (***2.3 Trivial*)
+         reflexivity.
+
+
+
+
+       - unfold CausCons. intros; rename η0 into η'; rename r0 into r'. rename H6 into Hreduct.
+         clear HWF_Union1 HWF_Union2 H HProg H0. rename H4 into HBO'. 
+         inversion Hreduct. subst.
+         remember (E A vis so sameobj) as Ex.
+         assert (Ex-hbo a η'). {
+           apply HBO'_HBO with
+           (Ex:=Ex)(Ex':= (E A' vis' so' sameobj'))(s:=ss0)
+                   (i:=ii0)(op:=opp)(η:=η)(r:=r)(θ:=θ');auto.
+           intro. intuition. subst. specialize (H9 a). apply H9 in H1.
+           destruct H1. 
+           subst.
+           (*apply hbo accyclic*)
+
+
+           
+           inversion HBO'; subst.
+           +SCase"single step".
+            inversion H.
+            *SSCase"from soo".
+             inversion H0 as [Hso' Hsameobj']; simpl in Hso'; simpl in Hsameobj'; clear H0.
+             apply t_step. simpl. unfold soo. left.  split.
+             (*1Proof of so*)
+             specialize (H14 a η'). apply H14 in Hso'.
+             inversion Hso'.
+             (*1.1 proof from  (so a η'0 \/ a = η'0) /\ η' = η*)
+             destruct H0. rewrite H4; clear H4.
+             inversion H0.
+             (*1.1.1 proof from  (so a η'0)*)
+             replace so with ((E A vis so sameobj)-so) in H4.
+             rewrite SO_Seq_General.
+             rewrite SO_Seq_General  in H4. specialize (H8 η'0).
+             assert (seq η'0 = seq η - 1). { assert (seq η'0 = ii0-1). intuition. rewrite H6. intuition. }
+             rewrite H6 in H4. omega. reflexivity.
+             (*1.1.2 proof from  (a = η'0)*)
+             apply SO_Seq_General. rewrite H4.
+             replace (seq η'0) with (ii0 - 1). replace (seq η) with ii0.
+             apply Theorem8_nat_help. (***!***) admit. (******!****)
+             intuition.  specialize (H8 η'0). intuition. 
+             (*1.2 proof from so: trivial*)
+             apply H0.
+
+             (*2proof of sameobj*)
+             apply Sameobj_Def with (Ex:= (E A vis so sameobj)) (Ex':=  (E A' vis' so' sameobj'))
+                                                                (opk :=  < ss0, ii0, opp >)
+                                                                (η:=η)(r:=r)(Θ:= θ'); simpl;auto.
+             apply WF_Relation with (a:=a)(b:=η')(r:=sameobj') in Hsameobj'.
+             destruct Hsameobj'. replace (sameobj') with ((E A' vis' so' sameobj')-sameobj) in H0;auto.
+             apply Sameobj_Domain in H0; simpl in H0.
+             replace (sameobj') with ((E A' vis' so' sameobj')-sameobj) in H4;auto.
+             apply Sameobj_Domain in H4; simpl in H4.
+(*here we need to prove that A a and A η'*)
+             specialize (H9 a).
+             apply H9 in H0. destruct H0; auto.
+             subst. intuition.
+             apply SO_NewEff with (Ex:= E A vis so sameobj) (Ex':=  E A' vis' so' sameobj')
+                                                                (opk :=  < ss0, ii0, opp >)
+                                                                (η:=η)(r:=r)(Θ:= θ')(a:=η') in Hreduct.
+             
+             
+         }
+
+
+
+                               
+         unfold CausCons in HCausCons. specialize (HCausCons r' a η').
+         apply HCausCons; auto.
+
+       -unfold CausCons. intros; rename η0 into η'; rename r0 into r'.
+         assert (Ex-hbo a η'). admit.
+         unfold CausCons in HCausCons. specialize (HCausCons r' a η').
+         apply HCausCons; auto.
